Module inclusion to reduce the number of dependencies while programming in Steel

examples/lowstar_permissions/Test.Array.fst
@@ -1,18 +1,15 @@
 module Test.Array
 
 module P = LowStar.Permissions
-module A = LowStar.RST.Array
-module Arr = LowStar.Array
 module RST = LowStar.RST
-module R = LowStar.Resource
-module HST = FStar.HyperStack.ST
+module A = LowStar.RST.Array
 
 
 #reset-options "--z3rlimit 10 --max_fuel 0 --max_ifuel 0 --z3cliopt smt.qi.eager_threshold=1000"
 #restart-solver
 let read_write_without_sharing () : RST.RST unit
-  (R.empty_resource)
-  (fun _ -> R.empty_resource)
+  (RST.empty_resource)
+  (fun _ -> RST.empty_resource)
   (fun _ -> True)
   (fun _ _ _ -> True)
   =
@@ -54,8 +51,8 @@ let read_write_without_sharing () : RST.RST unit
 
 #set-options "--z3rlimit 20"
 let read_write_with_sharing () : RST.RST unit
-  (R.empty_resource)
-  (fun _ -> R.empty_resource)
+  (RST.empty_resource)
+  (fun _ -> RST.empty_resource)
   (fun _ -> True)
   (fun _ _ _ -> True)
   =
@@ -65,46 +62,46 @@ let read_write_with_sharing () : RST.RST unit
   let b1 = A.share b in
   let x1 =
     RST.rst_frame
-      (R.(A.array_resource b <*> A.array_resource b1))
-      (fun _ -> R.(A.array_resource b <*> A.array_resource b1))
+      (RST.(A.array_resource b <*> A.array_resource b1))
+      (fun _ -> RST.(A.array_resource b <*> A.array_resource b1))
       (fun _ ->
         A.index b 0ul
       )
   in
   let b_first, b_second = RST.rst_frame
-    (R.(A.array_resource b <*> A.array_resource b1))
-    (fun p -> R.(A.array_resource (fst p) <*> A.array_resource (snd p) <*> A.array_resource b1))
+    (RST.(A.array_resource b <*> A.array_resource b1))
+    (fun p -> RST.(A.array_resource (fst p) <*> A.array_resource (snd p) <*> A.array_resource b1))
     (let f = fun _ -> A.split #FStar.UInt32.t b 1ul in f) //TODO: remove let binding
   in
     let h0 =
-    RST.get R.(A.array_resource b_first <*> A.array_resource b_second <*> A.array_resource b1)
+    RST.get RST.(A.array_resource b_first <*> A.array_resource b_second <*> A.array_resource b1)
   in
-  assert(A.get_perm b_first h0 == A.get_perm b_second h0);
+  assert(A.get_rperm b_first h0 == A.get_rperm b_second h0);
   let x2 = RST.rst_frame
-    (R.(A.array_resource b_first <*> A.array_resource b_second <*> A.array_resource b1))
-    (fun _ -> (R.(A.array_resource b_first <*> A.array_resource b_second <*> A.array_resource b1)))
+    (RST.(A.array_resource b_first <*> A.array_resource b_second <*> A.array_resource b1))
+    (fun _ -> (RST.(A.array_resource b_first <*> A.array_resource b_second <*> A.array_resource b1)))
     (fun _ -> A.index b_second 0ul)
   in
   let h1 =
-    RST.get R.(A.array_resource b_first <*> A.array_resource b_second <*> A.array_resource b1)
+    RST.get RST.(A.array_resource b_first <*> A.array_resource b_second <*> A.array_resource b1)
   in
   assume(
-    RST.focus_rmem h0 R.(A.array_resource b_first <*> A.array_resource b_second) ==
-    RST.focus_rmem h1 R.(A.array_resource b_first <*> A.array_resource b_second)
+    RST.focus_rmem h0 RST.(A.array_resource b_first <*> A.array_resource b_second) ==
+    RST.focus_rmem h1 RST.(A.array_resource b_first <*> A.array_resource b_second)
   );
   assume(
-    RST.focus_rmem h0 R.(A.array_resource b1) ==
-    RST.focus_rmem h1 R.(A.array_resource b1)
+    RST.focus_rmem h0 RST.(A.array_resource b1) ==
+    RST.focus_rmem h1 RST.(A.array_resource b1)
   );
   RST.rst_frame
-    (R.(A.array_resource b_first <*> A.array_resource b_second <*> A.array_resource b1))
-    (fun _ -> R.(A.array_resource b <*> A.array_resource b1))
+    (RST.(A.array_resource b_first <*> A.array_resource b_second <*> A.array_resource b1))
+    (fun _ -> RST.(A.array_resource b <*> A.array_resource b1))
     (fun _ -> A.glue b b_first b_second);
-  let h2 = RST.get R.(A.array_resource b <*> A.array_resource b1) in
+  let h2 = RST.get RST.(A.array_resource b <*> A.array_resource b1) in
   assume(
-    RST.focus_rmem h1 R.(A.array_resource b1) ==
-    RST.focus_rmem h2 R.(A.array_resource b1)
+    RST.focus_rmem h1 RST.(A.array_resource b1) ==
+    RST.focus_rmem h2 RST.(A.array_resource b1)
   );
   A.gather b b1;
-  let h = RST.get R.(A.array_resource b) in
+  let h = RST.get RST.(A.array_resource b) in
   A.free b
