ulib/LowStar.RST.Array.Views.fst
@@ -16,7 +16,6 @@
 module LowStar.RST.Array.Views
 
 open FStar.HyperStack.ST
-module A = LowStar.Array
 module HS = FStar.HyperStack
 module HST = FStar.HyperStack.ST
 module Seq = FStar.Seq
@@ -24,76 +23,81 @@ module P = LowStar.Permissions
 module MG = FStar.ModifiesGen
 module U32 = FStar.UInt32
 
-open LowStar.Resource
 open LowStar.RST
 
-noeq type varray (#a: Type) (b: A.array a) = {
-  s: Seq.lseq a (A.vlength b);
+include LowStar.Array
+
+noeq type varray (#a: Type) (b: array a) = {
+  s: Seq.lseq a (vlength b);
   p: Ghost.erased P.permission
 }
 
-let constant_perm_seq (#a: Type) (h: HS.mem) (b: A.array a) : Type =
-  (forall (i:nat{i < A.vlength b}) (j:nat{j < A.vlength b}). {:pattern (A.get_perm h b i); (A.get_perm h b j) }
-      A.get_perm h b i == A.get_perm h b j // Array resource cells have uniform permissions
+let constant_perm_seq (#a: Type) (h: HS.mem) (b: array a) : Type =
+  (forall (i:nat{i < vlength b}) (j:nat{j < vlength b}). {:pattern (get_perm h b i); (get_perm h b j) }
+      get_perm h b i == get_perm h b j // Array resource cells have uniform permissions
   )
 
-let same_perm_seq_always_constant (#a: Type) (h0 h1: HS.mem) (b:A.array a) : Lemma
-  (requires (A.as_perm_seq h0 b == A.as_perm_seq h1 b /\ constant_perm_seq h0 b))
+let same_perm_seq_always_constant (#a: Type) (h0 h1: HS.mem) (b:array a) : Lemma
+  (requires (as_perm_seq h0 b == as_perm_seq h1 b /\ constant_perm_seq h0 b))
   (ensures (constant_perm_seq h1 b))
   [SMTPat (constant_perm_seq h1 b); SMTPat (constant_perm_seq h0 b)]
   =
-  let aux (i:nat{i < A.vlength b}) (j:nat{j < A.vlength b}) : Lemma ( A.get_perm h1 b i == A.get_perm h1 b j) =
-    assert(A.get_perm h0 b i == A.get_perm h0 b j)
+  let aux (i:nat{i < vlength b}) (j:nat{j < vlength b}) : Lemma ( get_perm h1 b i == get_perm h1 b j) =
+    assert(get_perm h0 b i == get_perm h0 b j)
   in
   Classical.forall_intro_2 aux
 
 #set-options "--z3rlimit 20"
 
 abstract
-let array_view (#a:Type) (b:A.array a) : Tot (view (varray b)) =
+let array_view (#a:Type) (b:array a) : Tot (view (varray b)) =
   reveal_view ();
-  let fp = Ghost.hide (A.loc_array b) in
+  let fp = Ghost.hide (loc_array b) in
   let inv (h: HS.mem) : prop =
-    A.live h b /\ constant_perm_seq h b
+    live h b /\ constant_perm_seq h b
   in
-  let sel (h: HS.mem) : GTot (varray b) = { s = A.as_seq h b; p = Ghost.hide (A.get_perm h b 0) } in
+  let sel (h: HS.mem) : GTot (varray b) = { s = as_seq h b; p = Ghost.hide (get_perm h b 0) } in
   {
     fp = fp;
     inv = inv;
     sel = sel
   }
 
-unfold let array_resource (#a:Type) (b:A.array a) : Tot resource =
+unfold let array_resource (#a:Type) (b:array a) : Tot resource =
   as_resource (array_view b)
 
-let as_seq
+let as_rseq
   (#a: Type)
-  (b: A.array a)
+  (b: array a)
   (#r: resource{array_resource #a b `is_subresource_of` r})
-  (h: rmem r) : GTot (Seq.lseq a (A.vlength b))  =
+  (h: rmem r) : GTot (Seq.lseq a (vlength b)) =
   (h (array_resource b)).s
 
-let get_perm
+let get_rperm
   (#a: Type)
-  (b: A.array a)
+  (b: array a)
   (#r: resource{array_resource #a b `is_subresource_of` r})
   (h: rmem r) : GTot P.permission =
   Ghost.reveal (h (array_resource b)).p
 
 let reveal_array ()
   : Lemma (
-    (forall a (b:A.array a) .{:pattern as_loc (fp (array_resource b))}
-      as_loc (fp (array_resource b)) == A.loc_array b) /\
-      (forall a (b:A.array a) h .{:pattern inv (array_resource b) h}
-        inv (array_resource b) h <==> A.live h b /\ constant_perm_seq h b
+    (forall a (b:array a) .{:pattern as_loc (fp (array_resource b))}
+      as_loc (fp (array_resource b)) == loc_array b) /\
+      (forall a (b:array a) h .{:pattern inv (array_resource b) h}
+        inv (array_resource b) h <==> live h b /\ constant_perm_seq h b
       ) /\
-      (forall a (b:A.array a) h .{:pattern sel (array_view b) h}
-        sel (array_view b) h == { s = A.as_seq h b; p = Ghost.hide (A.get_perm h b 0) }
+      (forall a (b:array a) h .{:pattern sel (array_view b) h}
+        sel (array_view b) h == { s = as_seq h b; p = Ghost.hide (get_perm h b 0) }
       )
     ) =
   ()
 
 
-let summable_permissions (#a:Type) (b:A.array a) (b':A.array a) (h: rmem (array_resource b <*> array_resource b')) =
-  A.gatherable b b' /\
-  P.summable_permissions (get_perm b h) (get_perm b' h)
+let summable_permissions
+  (#a:Type)
+  (b:array a)
+  (b':array a)
+  (h: rmem (array_resource b <*> array_resource b')) =
+  gatherable b b' /\
+  P.summable_permissions (get_rperm b h) (get_rperm b' h)
