ulib/LowStar.Array.Defs.fsti
@@ -17,8 +17,9 @@ val array (a:Type0): Type0
 val length (#a:Type) (b:array a) : GTot (l:U32.t{U32.v l > 0})
 let vlength (#a:Type) (b:array a) : GTot pos = U32.v (length b)
 
-/// A array is viewed as an `FStar.Seq.seq`. However, since these arrays have permissions attached to them, `as_seq` is doubled by an
-/// `as_seq_perm` which returns the list of permission held by the array on each of its cells.
+/// A array is viewed as an `FStar.Seq.seq`. However, since these arrays have permissions attached
+/// to them, `as_seq` is doubled by an `as_seq_perm` which returns the list of permission held by
+/// the array on each of its cells.
 val as_seq (#a:Type) (h:HS.mem) (b:array a) : GTot (s:Seq.seq a{Seq.length s == vlength b})
 val as_perm_seq (#a:Type) (h:HS.mem) (b:array a) : GTot (s:Seq.seq P.permission{Seq.length s == vlength b})
 
@@ -29,7 +30,9 @@ let get (#a:Type) (h:HS.mem) (b:array a) (i:nat{i < vlength b}) : GTot a
 let get_perm (#a:Type) (h:HS.mem) (b:array a) (i:nat{i < vlength b}) : GTot P.permission
   = Seq.index (as_perm_seq h b) i
 
-/// Liveness is an abstract predicate, required or ensured by functions in `LowStar.Array`. As a helper to understand its behavior, one can view it as "the array is correctly allocated and all of its cells have a strictly positive permission".
+/// Liveness is an abstract predicate, required or ensured by functions in `LowStar.Array`.
+/// As a helper to understand its behavior, one can view it as "the array is correctly allocated
+/// and all of its cells have a strictly positive permission".
 val live (#a:Type) (h:HS.mem) (b:array a) : Type0
 
 /// Helpers for specifying full permissions on an array.
@@ -40,8 +43,8 @@ let writeable #a h b =
   (forall (i:nat{i < vlength #a b}). {:pattern (get_perm h b i) } writeable_cell h b i)
 
 
-/// Abstract predicate used to describe what happens after sharing an array to get two immutable references from it. It implies that the
-/// two arrays have the same length, and is commutative.
+/// Abstract predicate used to describe what happens after sharing an array to get two immutable
+/// references from it. It implies that the two arrays have the same length, and is commutative.
 val gatherable (#a:Type0) (b1 b2:array a) : Type0
 val gatherable_same_length (#a:Type0) (b1 b2:array a) : Lemma
   (requires (gatherable b1 b2))
@@ -75,7 +78,8 @@ val gsub (#a:Type0) (b:array a) (i:U32.t) (len:U32.t{U32.v len > 0})
 	   as_perm_seq h b' == Seq.slice (as_perm_seq h b) (U32.v i) (U32.v i + U32.v len)
 	 ))
 
-/// `gsub` enjoys various properties related to the view and the length of the sub-array, compared to the original array.
+/// `gsub` enjoys various properties related to the view and the length of the sub-array,
+/// compared to the original array.
 val live_gsub (#a:Type0) (h:HS.mem) (b:array a) (i:U32.t) (len:U32.t{U32.v len > 0})
   :Lemma (requires (U32.v i + U32.v len <= vlength b))
          (ensures  (live h b ==> (live h (gsub  b i len))))
@@ -87,11 +91,22 @@ val len_gsub (#a:Type0) (b:array a) (i:U32.t) (len':U32.t{U32.v len' > 0})
              [SMTPat (length (gsub b i len'))];
              [SMTPat (length (gsub b i len'))];
          ]]
-val gsub_inj (#a:Type0) (b1 b2:array a) (i1 i2:U32.t) (len1:U32.t{U32.v len1 > 0}) (len2:U32.t{U32.v len2 > 0})
-  :Lemma (requires (U32.v i1 + U32.v len1 <= vlength b1 /\
-                    U32.v i2 + U32.v len2 <= vlength b2 /\
-		    gsub b1 i1 len1 === gsub b2 i2 len2))
-         (ensures (len1 == len2 /\ (b1 == b2 ==> i1 == i2) /\ ((i1 == i2 /\ length b1 == length b2) ==> b1 == b2)))
+val gsub_inj
+  (#a:Type0)
+  (b1 b2:array a)
+  (i1 i2:U32.t)
+  (len1:U32.t{U32.v len1 > 0})
+  (len2:U32.t{U32.v len2 > 0})
+  : Lemma
+    (requires (
+      U32.v i1 + U32.v len1 <= vlength b1 /\
+      U32.v i2 + U32.v len2 <= vlength b2 /\
+      gsub b1 i1 len1 === gsub b2 i2 len2
+    ))
+    (ensures (
+      len1 == len2 /\ (b1 == b2 ==> i1 == i2) /\
+      ((i1 == i2 /\ length b1 == length b2) ==> b1 == b2)
+    ))
 val gsub_gsub (#a:Type0)
   (b:array a)
   (i1:U32.t) (len1:U32.t{U32.v len1 > 0})
@@ -104,6 +119,6 @@ val gsub_zero_length (#a:Type0) (b:array a)
   :Lemma (b == gsub  b 0ul (length b))
 
 
-/// There exists a more sophisticated form of sub-array extraction that involves splitting an array into two disjoint parts, and this is
-/// precisely what this abstract predicate captures.
+/// There exists a more sophisticated form of sub-array extraction that involves splitting an array
+/// into two disjoint parts, and this is precisely what this abstract predicate captures.
 val is_split_into (#a:Type0) (b: array a) (s:array a & array a) : Type0
